$\afcup(x)$
&
$\begin {array}{c}
\left[-2,2\right]\\
\int\limits_{-2}^2\afcup(x)=1\\
\afcup(0)=\int\limits_{-1}^1\up^2(x)dx
\end {array}$ & 
$\begin {array}{c}
y''(x)=2y(2x+2)-4y(2x)+2y(2x-2)\\
\widehat{\afcup}(t)=\prod\limits_{k=1}^{\infty}{\sinc^2\left(\frac{t}{2^{k}}\right)}=\prod\limits_{m=1}^{\infty}{\cos^{2m}(t\,2^{-m-1})}\\
\afcup(x)=\frac{1}{2}\left(\frac{1}{2}+\sum\limits_{k=1}^{\infty}\widehat{\afcup}(\frac{\pi k}{2})\cos(\frac{\pi k}{2} x)\right)%=%\\=\frac{1}{2}+\sum\limits_{k=1}^{\infty}\left(\left(\prod\limits_{m=1}^{\infty}{\cos^m(\frac{\pi k}{2^{m+1}})}\right)\cos(\pi k x)\right)
\end{array}$ 
& $\afcup(x)=\up(x)*\up(x)$
 & w e

%$\up(x)=\frac{1}{2\pi}\int\limits_{-\infty}^{\infty}e^{itx}\prod\limits_{k=1}^{\infty}\frac{\sin(t\,2^{-k})}{t\,2^{-k}}dt$\\

%$\widehat{\up}(t)=\prod\limits_{k=1}^{\infty}\frac{\sin(t\,2^{-k})}{t\,2^{-k}}=\prod\limits_{k=1}^{\infty}{\sinc(t\,2^{-k})}=\prod\limits_{m=1}^{\infty}{\cos^m(t\,2^{-m-1})}$  Книга про антенны стр 37.\quad $\sinc(x)=\prod\limits_{k=1}^{\infty}\cos(2^{-k}x)$ зеленая кн. стр 23\\
%Тогда $\up(x)=\frac{1}{2}+\sum\limits_{k=1}^{\infty}\widehat{\up}(\pi k)\cos(\pi k x)=\frac{1}{2}+\sum\limits_{k=1}^{\infty}\left(\left(\prod\limits_{m=1}^{\infty}{\cos^m(\frac{\pi k}{2^{m+1}})}\right)\cos(\pi k x)\right)$.

