$\begin{array}{c}
\mathrm{eup}_{a}\\\\ (y_k,\,\mathrm{pe})
\end{array}$&
$\begin{array}{c}
\left[-1,\,1\right]\\\\
\int\limits_{-1}^{1} \mathrm{eup}_{a}(x)=1
\end{array}$ &
$\begin{array}{c}
y'(x) - \ln{(a)}\,y(x) = \dfrac{\ln{(a)}}{a-1}(y(2x+1)-a y(2x-1))\\[6pt]
\widehat{\mathrm{eup}_{a}}(t)=\prod\limits_{k=1}^{\infty}{\biggl(\dfrac{\shc(\ln(a)/2-\I\,t\,2^{-k})}{\shc(\ln(a)/2)}\biggr)}\\[6pt]
\mathrm{eup}_{a}(x)=\dfrac{1}{2}+\sum\limits_{k=1}^{\infty}\Re(\widehat{\mathrm{eup}_{a}}(k\pi))\cos(k\pi x) - \\
\Im(\widehat{\mathrm{eup}_{a}}(k\pi))\sin(k\pi x) \\
\sum\limits_{k\in\mathbb{Z}}a^k\,\eup_a(x-k) \equiv a^x \eup_a(0)
\end{array}$
&
q
& 
\begin{tabular}{c}
w e \\ \cite{ncls}\\ \cite{Gor94}
\end{tabular}
