$\fip_{a,n}(x)$&
$\begin {array}{c}
\left[-\frac{l}{2};\frac{l}{2}\right],~
l=n+\frac{2}{a-1}\\
\int\limits_{\supp}\!\!\fip_{a,n}(x)=1\\
\fip_{a,n}(0)=?
\end {array}$& 
$\begin {array}{c}
\widehat{\fip_{a,m}}(t)=
\sinc{\left(\frac{t}{2}\right)}^n\cdot
\prod_{k=1}^{\infty}\sinc{\left(t\cdot a^{-k}\right)}\\
\fip_{a,n}=
\frac{2}{l}\left(
\frac{1}{2}+
\sum\limits_{k=1}^{\infty}\widehat{\fip_{a,n}}\left(\frac{2\pi k}{l}\right)\cos\left(\frac{2\pi kx}{l}\right)
\right)
\end{array}$ 
& 
$
\begin {array}{c}
\fip_{2,0}(x)\equiv\up_n(x)\\
\fip_{2,n}(x)\equiv\fup_n(x)\\
\fip_{a,0}(x)\equiv\ha(x)\\
\fip_{a,n}(x) = \ha(x)\ast\Theta_{n-1}(x)
\end{array}$
& 

\cite{Br18}

%$\up(x)=\frac{1}{2\pi}\int\limits_{-\infty}^{\infty}e^{itx}\prod\limits_{k=1}^{\infty}\frac{\sin(t\,2^{-k})}{t\,2^{-k}}dt$\\

%$\widehat{\up}(t)=\prod\limits_{k=1}^{\infty}\frac{\sin(t\,2^{-k})}{t\,2^{-k}}=\prod\limits_{k=1}^{\infty}{\sinc(t\,2^{-k})}=\prod\limits_{m=1}^{\infty}{\cos^m(t\,2^{-m-1})}$  Книга про антенны стр 37.\quad $\sinc(x)=\prod\limits_{k=1}^{\infty}\cos(2^{-k}x)$ зеленая кн. стр 23\\
%Тогда $\up(x)=\frac{1}{2}+\sum\limits_{k=0}^{\infty}\widehat{\up}(\pi k)\cos(\pi k x)=\frac{1}{2}+\sum\limits_{k=0}^{\infty}\left(\left(\prod\limits_{m=1}^{\infty}{\cos^m(\frac{\pi k}{2^{m+1}})}\right)\cos(\pi k x)\right)$.

