$\fp_{m,n}(x)$&
$\begin {array}{c}
\left[-\frac{n+2}{2};\frac{n+2}{2}\right]\\
\int\limits_{\supp}\!\!\fp_{m,n}(x)=1\\
\fp_{m,n}(0)=?
\end {array}$& 
$\begin {array}{c}
\widehat{\fp_{n,m}}(t)=
\sinc{\left(\frac{t}{2}\right)}^n\cdot
\widehat{\up_m}{\left(t\right)}\\
\fp_{m,n}=
\frac{2}{n+2}\left(
\frac{1}{2}+
\sum\limits_{k=1}^{\infty}\widehat{\fp_{m,n}}\left(\frac{2\pi k}{n+2}\right)\cos\left(\frac{2\pi kx}{n+2}\right)
\right)
\end{array}$ 
& 
$\begin {array}{c}
\fup_{m,0}(x)\equiv\up_m(x)\\
\fup_{m,m}(x) = \up_m(x)\ast\Theta_{n-1}(x)\\
\end{array}$
& 

\cite{Br18}

%$\up(x)=\frac{1}{2\pi}\int\limits_{-\infty}^{\infty}e^{itx}\prod\limits_{k=1}^{\infty}\frac{\sin(t\,2^{-k})}{t\,2^{-k}}dt$\\

%$\widehat{\up}(t)=\prod\limits_{k=1}^{\infty}\frac{\sin(t\,2^{-k})}{t\,2^{-k}}=\prod\limits_{k=1}^{\infty}{\sinc(t\,2^{-k})}=\prod\limits_{m=1}^{\infty}{\cos^m(t\,2^{-m-1})}$  Книга про антенны стр 37.\quad $\sinc(x)=\prod\limits_{k=1}^{\infty}\cos(2^{-k}x)$ зеленая кн. стр 23\\
%Тогда $\up(x)=\frac{1}{2}+\sum\limits_{k=0}^{\infty}\widehat{\up}(\pi k)\cos(\pi k x)=\frac{1}{2}+\sum\limits_{k=0}^{\infty}\left(\left(\prod\limits_{m=1}^{\infty}{\cos^m(\frac{\pi k}{2^{m+1}})}\right)\cos(\pi k x)\right)$.

