$\Fup_n(x)$&
$\begin {array}{c}
\left[-\frac{n+2}{2^n};\frac{n+2}{2^n}\right]\\
\int\limits_{\supp}\!\!\Fup_n(x)=1\\
\Fup_n(0)=?
\end {array}$ & 
$\begin {array}{c}
y'(x)=2\sum\limits_{k=0}^{n+2}\left(C_{n+1}^{k}-C_{n+1}^{k-1}\right)
y\!\left(2x-\frac{2(k-1)-n}{2^{n+2}}\right)\\
\widehat{\Fup_n}(t)=
\left(\sinc\left(t\cdot2^{-n-1}\right)\right)^{n+1}\cdot\prod
\limits_{k=1}^{\infty}\sinc\left(t\cdot2^{-k}\right)%\\
%\fup_n=\frac{2}{n+2}\left(\frac{1}{2}+\sum\limits_{k=1}^{\infty}\widehat{\fup_n}\left(\frac{2\pi k}{n+2}\right)\cos\left(\frac{2\pi kx}{n+2}\right)\right)
\end{array}$ 
& 
$
\begin{array}{c}
\Fup_n(x) = \\2^{C_{n+1}^2}\up{\left(x-1+(n+2)2^{-n-1}\right)}
\end{array}
$
%$\begin {array}{c}
%\fup_0(x)\equiv\up(x)\\ 
%\fup_n(x)=2\up(2x)*\Theta_n(x)\\
%\fup_n(x)=\up(x)*\Theta_{n-1}(x)
%\end{array}$
& \cite{Got99} \cite{Ba08} 

%$\up(x)=\frac{1}{2\pi}\int\limits_{-\infty}^{\infty}e^{itx}\prod\limits_{k=1}^{\infty}\frac{\sin(t\,2^{-k})}{t\,2^{-k}}dt$\\

%$\widehat{\up}(t)=\prod\limits_{k=1}^{\infty}\frac{\sin(t\,2^{-k})}{t\,2^{-k}}=\prod\limits_{k=1}^{\infty}{\sinc(t\,2^{-k})}=\prod\limits_{m=1}^{\infty}{\cos^m(t\,2^{-m-1})}$  Книга про антенны стр 37.\quad $\sinc(x)=\prod\limits_{k=1}^{\infty}\cos(2^{-k}x)$ зеленая кн. стр 23\\
%Тогда $\up(x)=\frac{1}{2}+\sum\limits_{k=0}^{\infty}\widehat{\up}(\pi k)\cos(\pi k x)=\frac{1}{2}+\sum\limits_{k=0}^{\infty}\left(\left(\prod\limits_{m=1}^{\infty}{\cos^m(\frac{\pi k}{2^{m+1}})}\right)\cos(\pi k x)\right)$.

