$\fup_n(x)$&
$\begin {array}{c}
\left[-\frac{n+2}{2};\frac{n+2}{2}\right]\\
\int\limits_{\supp}\!\!\fup_n(x)=1\\
\fup_n(0)=?
\end {array}$ & 
$\begin {array}{c}
%\fup_n'(x)=\frac{1}{2^{n-1}}\sum\limits_{k=0}^{n+2}\left(C_{n+1}^{k}-C_{n+1}^{k-1}\right)\fup_n\!\left(2x+\frac{n+2}{2}-k\right)\\
y'(x)=\frac{1}{2^{n-1}}\sum\limits_{k=0}^{n+2}\left(C_{n+1}^{k}-C_{n+1}^{k-1}\right)y\!\left(2x+\frac{n+2}{2}-k\right)\\
\widehat{\fup_n}(t)=\left(\sinc\left(\frac{t}{2}\right)\right)^n\cdot\prod\limits_{k=1}^{\infty}\sinc\left(\frac{t}{2^k}\right)=\\=\left(\sinc\left(\frac{t}{2}\right)\right)^{n+1}\cdot\prod\limits_{k=2}^{\infty}\sinc\left(\frac{t}{2^k}\right)\\
\fup_n=\frac{2}{n+2}\left(\frac{1}{2}+\sum\limits_{k=1}^{\infty}\widehat{\fup_n}\left(\frac{2\pi k}{n+2}\right)\cos\left(\frac{2\pi kx}{n+2}\right)\right)
\end{array}$ 
& $\begin {array}{c}
\fup_0(x)\equiv\up(x)\\ 
\fup_n(x)=2\up(2x)*\Theta_n(x)\\
\fup_n(x)=\up(x)*\Theta_{n-1}(x)
\end{array}$
& w e

%$\up(x)=\frac{1}{2\pi}\int\limits_{-\infty}^{\infty}e^{itx}\prod\limits_{k=1}^{\infty}\frac{\sin(t\,2^{-k})}{t\,2^{-k}}dt$\\

%$\widehat{\up}(t)=\prod\limits_{k=1}^{\infty}\frac{\sin(t\,2^{-k})}{t\,2^{-k}}=\prod\limits_{k=1}^{\infty}{\sinc(t\,2^{-k})}=\prod\limits_{m=1}^{\infty}{\cos^m(t\,2^{-m-1})}$  Книга про антенны стр 37.\quad $\sinc(x)=\prod\limits_{k=1}^{\infty}\cos(2^{-k}x)$ зеленая кн. стр 23\\
%Тогда $\up(x)=\frac{1}{2}+\sum\limits_{k=0}^{\infty}\widehat{\up}(\pi k)\cos(\pi k x)=\frac{1}{2}+\sum\limits_{k=0}^{\infty}\left(\left(\prod\limits_{m=1}^{\infty}{\cos^m(\frac{\pi k}{2^{m+1}})}\right)\cos(\pi k x)\right)$.

