$\Fup_{m,n}(x)$&
q & 
$\begin {array}{c}
\widehat{\Fup_{n,m}}(t)=
\sinc{\left(\frac{t}{2(2m)^n}\right)}^{n}\cdot
\widehat{\up_m}\left(\frac{t}{2(2m)^n}\right)%\\
%\fup_n=\frac{2}{n+2}\left(\frac{1}{2}+\sum\limits_{k=1}^{\infty}\widehat{\fup_n}\left(\frac{2\pi k}{n+2}\right)\cos\left(\frac{2\pi kx}{n+2}\right)\right)
\end{array}$ 
& 
q
%$\begin {array}{c}
%\fup_0(x)\equiv\up(x)\\ 
%\fup_n(x)=2\up(2x)*\Theta_n(x)\\
%\fup_n(x)=\up(x)*\Theta_{n-1}(x)
%\end{array}$
& \cite{Br18}

%$\up(x)=\frac{1}{2\pi}\int\limits_{-\infty}^{\infty}e^{itx}\prod\limits_{k=1}^{\infty}\frac{\sin(t\,2^{-k})}{t\,2^{-k}}dt$\\

%$\widehat{\up}(t)=\prod\limits_{k=1}^{\infty}\frac{\sin(t\,2^{-k})}{t\,2^{-k}}=\prod\limits_{k=1}^{\infty}{\sinc(t\,2^{-k})}=\prod\limits_{m=1}^{\infty}{\cos^m(t\,2^{-m-1})}$  Книга про антенны стр 37.\quad $\sinc(x)=\prod\limits_{k=1}^{\infty}\cos(2^{-k}x)$ зеленая кн. стр 23\\
%Тогда $\up(x)=\frac{1}{2}+\sum\limits_{k=0}^{\infty}\widehat{\up}(\pi k)\cos(\pi k x)=\frac{1}{2}+\sum\limits_{k=0}^{\infty}\left(\left(\prod\limits_{m=1}^{\infty}{\cos^m(\frac{\pi k}{2^{m+1}})}\right)\cos(\pi k x)\right)$.

