$\begin{array}{c}
\g_{k,h}\\\\ (y_{\omega,h})
\end{array}$&
$\begin{array}{c}
\left[-h,\,h\right]\\\\
\int\limits_{-h}^{h} \mathrm{\g}_{k,h}(x)=1
\end{array}$ &
$\begin{array}{c}
y''(x) + k^2y(x) = ay(3x+2h)-by(3x)+ay(3x-2h)\\[6pt]
a = \dfrac{3}{2}\cdot\dfrac{k^2}{1-\cos(2kh/3)},\,b=2a\cos\biggl(\frac{2kh}{3}\biggr)\\[6pt]
\widehat{\mathrm{g}_{k,h}}(t)=\prod\limits_{j=1}^{\infty}{\dfrac{2a}{3}\dfrac{\cos(2th\cdot3^{-j})-\cos(2th\cdot3^{-1})}{k^2 - t^29^{1-j}}}\\[6pt]
\mathrm{g}_{k,h}(x) = \sum\limits_{k=1}^{\infty}\widehat{\mathrm{g}_{k,h}}(k\pi))(\cos(k\pi x) - \cos(k\pi))\\
\sin(kx) = d_1 \sum\limits_{j\in\mathbb{Z}}\sin\biggl(\dfrac{2khj}{3}\biggr)\,\g_{k,h}\biggl(x-\dfrac{2hj}{3}\biggr) \\
d_1 = \dfrac{\pi^2}{2k\sin{\frac{2kh}{3}}\g_{k,h}'(-\frac{2h}{3})} \\
\cos(kx) = d_2 \sum\limits_{j\in\mathbb{Z}}\cos\biggl(\dfrac{2khj}{3}\biggr)\,\g_{k,h}\biggl(x-\dfrac{2hj}{3}\biggr) \\
d_2 = \dfrac{1}{\g_{k,h}(0)+2\cos{\frac{2kh}{3}}\g_{k,h}(-\frac{2h}{3})} \\
\end{array}$
&
q
&
\begin{tabular}{c}
w e \\ \cite{ncls}\\ \cite{Got99}
\end{tabular}
