${\mathrm h}_a(x)$&
$\begin {array}{c}
\left[-\frac{1}{a-1},\frac{1}{a-1}\right]\\
\int\limits_{\supp}\!\!{\mathrm h}_a(x)=1\\
{\mathrm h}_a(0)=\frac{a}{2},\,\,\, a\geqslant2
\end {array}$ & 
$\begin {array}{c}
y'(x)=\frac{a^2}{2}\left(\rule{0pt}{10pt}y(ax+1)-y(ax-1)\right)\\
\widehat{{\mathrm h}_a}(t)=\prod\limits_{k=1}^{\infty}{\sinc\left(\frac{t}{a^{k}}\right)}%=\prod\limits_{m=1}^{\infty}{\cos^m(t\,2^{-m-1})}
\\
{\mathrm h}_a(x)=(a-1)\left(\frac{1}{2}+\sum\limits_{k=1}^{\infty}\widehat{{\mathrm h}_a}\!\left(\rule{0pt}{10pt}(a-1)\pi k\right)\cos\!\left(\rule{0pt}{10pt}(a-1)\pi kx\right)\right)%=\\=\frac{1}{2}+\sum\limits_{k=1}^{\infty}\left(\left(\prod\limits_{m=1}^{\infty}{\cos^m(\frac{\pi k}{2^{m+1}})}\right)\cos(\pi k x)\right)
\end{array}$
& 
${\mathrm h}_2(x)\equiv\up(x)$
& [1]

%$\up(x)=\frac{1}{2\pi}\int\limits_{-\infty}^{\infty}e^{itx}\prod\limits_{k=1}^{\infty}\frac{\sin(t\,2^{-k})}{t\,2^{-k}}dt$\\

%$\widehat{\up}(t)=\prod\limits_{k=1}^{\infty}\frac{\sin(t\,2^{-k})}{t\,2^{-k}}=\prod\limits_{k=1}^{\infty}{\sinc(t\,2^{-k})}=\prod\limits_{m=1}^{\infty}{\cos^m(t\,2^{-m-1})}$  Книга про антенны стр 37.\quad $\sinc(x)=\prod\limits_{k=1}^{\infty}\cos(2^{-k}x)$ зеленая кн. стр 23\\
%Тогда $\up(x)=\frac{1}{2}+\sum\limits_{k=1}^{\infty}\widehat{\up}(\pi k)\cos(\pi k x)=\frac{1}{2}+\sum\limits_{k=1}^{\infty}\left(\left(\prod\limits_{m=1}^{\infty}{\cos^m(\frac{\pi k}{2^{m+1}})}\right)\cos(\pi k x)\right)$.

