$\pi_m(x)$&
$\begin {array}{c}
\left[-1,1\right]\\
\int\limits_{-1}^1\pi_m(x)=1\\
\max(\pi_m)=\frac{2m}{3m-2}\\
\pi_m(0)=\\\!\!\left\{\!\!
\begin{array}{cc}
\frac{2m}{3m-2}&m\mbox{ - четное},\\
\frac{m}{3m-2}&m\mbox{ - нечетное}.
\end{array}
\right.\!\!\!\!
\end {array}$ & 
$\begin {array}{c}
y'=\frac{2m^2}{3m-2}\left(\rule{0pt}{15pt}\right.\!\!%(%\left((
y(2mx+2m-1)+\\+\sum\limits_{k=2}^{2m-1}(-1)^ky(2mx+2m-2k+1)-y(2mx-2m+1)
\!\!\left)\rule{0pt}{15pt}\right.%)%\right)
\\
\widehat{\pi_m}(t)=\prod\limits_{k=1}^{\infty}P\left(\frac{t}{(2m)^k}\right),\quad\mbox{где}\quad
P(t)=\\\frac{1}{3m-2}\left((m-1)\frac{\mathrm{sinc}(t)\mathrm{sinc}(2(m-1)t)}{\mathrm{sinc}(2t)}+(2m-1)\mathrm{sinc}((2m-1)t)\right)\\
\pi_m(x)=\frac{1}{2}+\sum\limits_{k=1}^{\infty}\widehat{\pi_m}(\pi k)\cos(\pi k x)
\end{array}$ 
&
$\begin{array}{c}
\pi_1(x)\equiv\up(x)\\
\pi_2(x)\equiv\up_2(x)
\end{array}$
&
\cite{KVF2003}