$\begin{array}{c}
\up(x)\\[4pt] (\HilbergsHut)
\end{array}$&
$\begin {array}{c}
\left[-1,1\right]\\
\int\limits_{-1}^1\up(x)=1\\
\up(0)=1
\end {array}$ & 
$\begin {array}{c}
y'(x)=2y(2x+1)-2y(2x-1)\\
\widehat{\up}(t)=\prod\limits_{k=1}^{\infty}{\sinc\left(\frac{t}{2^{k}}\right)}=\prod\limits_{m=1}^{\infty}{\cos^m(t\,2^{-m-1})}\\
\up(x)=\frac{1}{2}+\sum\limits_{k=1}^{\infty}\widehat{\up}(\pi k)\cos(\pi k x)=\\=\frac{1}{2}+\sum\limits_{k=1}^{\infty}\left(\left(\prod\limits_{m=1}^{\infty}{\cos^m(\frac{\pi k}{2^{m+1}})}\right)\cos(\pi k x)\right)
\end{array}$
& q & w e

%$\up(x)=\frac{1}{2\pi}\int\limits_{-\infty}^{\infty}e^{itx}\prod\limits_{k=1}^{\infty}\frac{\sin(t\,2^{-k})}{t\,2^{-k}}dt$\\

%$\widehat{\up}(t)=\prod\limits_{k=1}^{\infty}\frac{\sin(t\,2^{-k})}{t\,2^{-k}}=\prod\limits_{k=1}^{\infty}{\sinc(t\,2^{-k})}=\prod\limits_{m=1}^{\infty}{\cos^m(t\,2^{-m-1})}$  Книга про антенны стр 37.\quad $\sinc(x)=\prod\limits_{k=1}^{\infty}\cos(2^{-k}x)$ зеленая кн. стр 23\\
%Тогда $\up(x)=\frac{1}{2}+\sum\limits_{k=1}^{\infty}\widehat{\up}(\pi k)\cos(\pi k x)=\frac{1}{2}+\sum\limits_{k=1}^{\infty}\left(\left(\prod\limits_{m=1}^{\infty}{\cos^m(\frac{\pi k}{2^{m+1}})}\right)\cos(\pi k x)\right)$.

