$\up_m(x)$&
$\begin {array}{c}
\left[-1,1\right]\\
\int\limits_{-1}^1\up_m(x)=1\\
\up_m(0)=1
\end {array}$ & 
$\begin {array}{c}
y'(x)=2\sum\limits_{k=1}^m\left(y(2mx+2m-2k+1)-y(2mx-2k+1)\right)\\
\widehat{\up_m}(t)=\prod\limits_{k=1}^{\infty}\frac{\sin^2\left(\frac{mt}{(2m)^k}\right)}{\frac{mt}{(2m)^k}\,m\, \sin\left(\frac{t}{(2m)^k}\right)}=\prod\limits_{k=1}^{\infty}\frac{\sinc^2\left(\frac{mt}{(2m)^k}\right)}{\sinc\left(\frac{t}{(2m)^k}\right)}\\
\up_m(x)=\frac{1}{2}+\sum\limits_{k=1}^{\infty}\widehat{\up_m}(\pi k)\cos(\pi k x)
\end{array}$ 
& $\up_1(x)\equiv\up(x)$ &Старец

%$\up(x)=\frac{1}{2\pi}\int\limits_{-\infty}^{\infty}e^{itx}\prod\limits_{k=1}^{\infty}\frac{\sin(t\,2^{-k})}{t\,2^{-k}}dt$\\

%$\widehat{\up}(t)=\prod\limits_{k=1}^{\infty}\frac{\sin(t\,2^{-k})}{t\,2^{-k}}=\prod\limits_{k=1}^{\infty}{\sinc(t\,2^{-k})}=\prod\limits_{m=1}^{\infty}{\cos^m(t\,2^{-m-1})}$  Книга про антенны стр 37.\quad $\sinc(x)=\prod\limits_{k=1}^{\infty}\cos(2^{-k}x)$ зеленая кн. стр 23\\
%Тогда $\up(x)=\frac{1}{2}+\sum\limits_{k=1}^{\infty}\widehat{\up}(\pi k)\cos(\pi k x)=\frac{1}{2}+\sum\limits_{k=1}^{\infty}\left(\left(\prod\limits_{m=1}^{\infty}{\cos^m(\frac{\pi k}{2^{m+1}})}\right)\cos(\pi k x)\right)$.

