$\Xi_n(x)$&
$\begin {array}{c}
\left[-1,1\right]\\
\int\limits_{-1}^1\Xi_n(x)=1
\end {array}$ & 
$\begin {array}{c}
y^{(n)}(x)=(n+1)^{n+1}2^{-n}\sum\limits_{k=0}^nC_n^k(-1)^ky((n+1)x+n-2k)\\
\widehat{\Xi_n}(t)=\prod\limits_{k=1}^{\infty}{\sinc^n\left(\frac{t}{(n+1)^{k}}\right)}\\
\Xi_n(x)=\frac{1}{2}+\sum\limits_{k=1}^{\infty}\widehat{\Xi_n}(\pi k)\cos(\pi k x)%=\\=\frac{1}{2}+\sum\limits_{k=1}^{\infty}\left(\left(\prod\limits_{m=1}^{\infty}{\cos^m(\frac{\pi k}{2^{m+1}})}\right)\cos(\pi k x)\right)
\end{array}$
& 
$\begin {array}{c}
\Xi_1\equiv\up(x)\\
\Xi_n=\underbrace{{\mathrm h}_{n+1}*\dots*{\mathrm h}_{n+1}}_n\\
\end{array}$
& [1]

%$\up(x)=\frac{1}{2\pi}\int\limits_{-\infty}^{\infty}e^{itx}\prod\limits_{k=1}^{\infty}\frac{\sin(t\,2^{-k})}{t\,2^{-k}}dt$\\

%$\widehat{\up}(t)=\prod\limits_{k=1}^{\infty}\frac{\sin(t\,2^{-k})}{t\,2^{-k}}=\prod\limits_{k=1}^{\infty}{\sinc(t\,2^{-k})}=\prod\limits_{m=1}^{\infty}{\cos^m(t\,2^{-m-1})}$  Книга про антенны стр 37.\quad $\sinc(x)=\prod\limits_{k=1}^{\infty}\cos(2^{-k}x)$ зеленая кн. стр 23\\
%Тогда $\up(x)=\frac{1}{2}+\sum\limits_{k=1}^{\infty}\widehat{\up}(\pi k)\cos(\pi k x)=\frac{1}{2}+\sum\limits_{k=1}^{\infty}\left(\left(\prod\limits_{m=1}^{\infty}{\cos^m(\frac{\pi k}{2^{m+1}})}\right)\cos(\pi k x)\right)$.

